Use a single environment everywhere for etp and relatives
This forbids cheating when proving that expression subtyping means value
subtyping. To do that, we must be able to turn (closed) values into expressions
with a valid environment, and the easiest way is to turn closed values into
closed expressions. But that requires changes to the syntax!

ecoop17/dot_wfrel2.v
@@ -210,19 +210,19 @@ Proof.
   intros * H; induction H; simpl; congruence.
 Qed.
 
-Program Definition etp T k env1 e env :=
-  @expr_sem k (fun k _ => vtp T k) k _ env1 e env.
+Program Definition etp T k e env :=
+  @expr_sem k (fun k _ => vtp T k) k _ env e env.
 
 (* Semantic typing *)
 Definition sem_type (G : tenv) (T : ty) (e: tm) :=
   forall k env,
     R_env k env G ->
-    etp T k env e env.
+    etp T k e env.
 
 Definition sem_subtype (G : tenv) (T1 T2: ty) :=
-  forall k env env1,
+  forall k env,
     R_env k env G ->
-    forall e, etp T1 k env1 e env -> etp T2 k env1 e env.
+    forall e, etp T1 k e env -> etp T2 k e env.
 
 Definition sem_vl_subtype (G : tenv) (T1 T2: ty) :=
   forall k env,
@@ -412,8 +412,8 @@ Ltac step_eval := n_is_succ; simpl in *.
 (* and e2 succeeds. That should be an exercise on some tactic like inv_mbind. *)
 
 (* We want to relate etp and vtp. *)
-Lemma etp_vtp_j: forall e v k j nm T env env1,
-    tevalSnm env1 e v j nm -> etp T k env1 e env -> j <= k -> vtp T (k - j) v env.
+Lemma etp_vtp_j: forall e v k j nm T env,
+    tevalSnm env e v j nm -> etp T k e env -> j <= k -> vtp T (k - j) v env.
 Proof.
   intros;
   assert (exists v0, Some v = Some v0 /\ vtp T (k - j) v0 env) by eauto;
@@ -421,34 +421,34 @@ Proof.
 Qed.
 Hint Resolve etp_vtp_j.
 
-Lemma etp_vtp: forall e v k nm T env env1,
-    tevalSnm env1 e v 0 nm -> etp T k env1 e env -> vtp T k v env.
+Lemma etp_vtp: forall e v k nm T env,
+    tevalSnm env e v 0 nm -> etp T k e env -> vtp T k v env.
 Proof. eauto. Qed.
 Hint Resolve etp_vtp.
 
-Lemma vtp_etp_j: forall e v T env env1 k j nm,
+Lemma vtp_etp_j: forall e v T env k j nm,
     vtp T (k - j) v env ->
-    tevalSnm env1 e v j nm ->
+    tevalSnm env e v j nm ->
     j <= k ->
-    etp T k env1 e env.
+    etp T k e env.
 Proof.
   intros * Hvtp Heval Hkj.
   unfold etp; vtp_unfold_pieces; unfold tevalSnOpt, tevalSnm in *.
   intros * [nm' Heval'] Hkj0.
   assert (optV = Some v /\ j = j0) as [-> ->] by (
     pose (N := nm + nm' + 1);
-    assert (tevalS e N env1 = Some (Some v, j)) by (subst N; auto);
-    assert (tevalS e N env1 = Some (optV, j0)) by (subst N; auto);
+    assert (tevalS e N env = Some (Some v, j)) by (subst N; auto);
+    assert (tevalS e N env = Some (optV, j0)) by (subst N; auto);
     split_conj; congruence);
   eexists; split_conj; eauto.
 Qed.
 Hint Resolve vtp_etp_j.
 
 Lemma vtp_etp:
-  forall e v T env env1 k nm,
+  forall e v T env k nm,
     vtp T k v env ->
-    tevalSnm env1 e v 0 nm ->
-    etp T k env1 e env.
+    tevalSnm env e v 0 nm ->
+    etp T k e env.
 Proof. eauto. Qed.
 Hint Resolve vtp_etp.
 
@@ -458,7 +458,8 @@ Proof.
   unfold sem_subtype, sem_vl_subtype.
   intros * H * Henv * HvT1.
   destruct (vl_to_tm v) as [[e env1] Heval]; eauto.
-Qed.
+Admitted.
+(* Qed. *)
 Hint Resolve subtype_to_vl_subtype.
 
 Lemma vl_sub_equiv: sem_subtype = sem_vl_subtype.
@@ -493,10 +494,10 @@ Admitted.
 Hint Immediate vtp_extend.
 
 Lemma vtp_etp_rev:
-  forall e v T env env1 k nm,
-    tevalSnm env1 e v 0 nm ->
+  forall e v T env k nm,
+    tevalSnm env e v 0 nm ->
     vtp T k v env ->
-    etp T k env1 e env.
+    etp T k e env.
   eauto. Qed.
 
 Lemma t_forall_i: forall G T1 T2 t,
@@ -538,7 +539,7 @@ Qed.
 Hint Resolve teval_var.
 
 Lemma etp_var: forall env x T n,
-  etp T n env (tvar x) env ->
+  etp T n (tvar x) env ->
   exists v,
     indexr x env = Some v /\
     vtp T n v env.
@@ -564,7 +565,7 @@ Qed.
 
 (* Better version of mem_stp. *)
 Lemma mem_stp_etp : forall env x L U n vx,
-    etp (TMem L U) (S n) env (tvar x) env ->
+    etp (TMem L U) (S n) (tvar x) env ->
     vtp L n vx env ->
     vtp (TSel (varF x)) (S n) vx env.
 Proof.
@@ -578,7 +579,7 @@ Proof.
 Qed.
 
 Lemma stp_mem_etp : forall env x L U n vx,
-    etp (TMem L U) (S n) env (tvar x) env ->
+    etp (TMem L U) (S n) (tvar x) env ->
     vtp (TSel (varF x)) (S n) vx env ->
     vtp U n vx env.
 Proof.
